clean up Parser file

coq/Parser.v
@@ -455,9 +455,80 @@ Proof.
   firstorder.
 Qed.
 
-(* The stack symbols that have already been processed represent
-   a (partial) derivation; this predicate relates those symbols
-   to the word (prefix) involved in the derivation. *)
+(* AN INVARIANT THAT RELATES "UNAVAILABLE" NONTERMINALS
+   TO THE SHAPE OF THE STACK *)
+
+Definition unavailable_nts_invar g st : Prop :=
+  match st with
+  | Pst av stk _ =>
+    unavailable_nts_are_open_calls g av (lstackOf stk)
+  end.
+
+Lemma unavailable_nts_invar_starts_true :
+  forall g ys ts,
+    unavailable_nts_invar g (mkInitState g ys ts).
+Proof.
+  intros g ys ts; unfold mkInitState; unfold unavailable_nts_are_open_calls.
+  intros x hi hn; ND.fsetdec.
+Qed.
+
+Lemma return_preserves_unavailable_nts_invar :
+  forall g av fr cr cr' frs o o' pre pre' x suf' v v' v'',
+    fr     = Fr (Loc o pre []) v
+    -> cr  = Fr (Loc o' pre' (NT x :: suf')) v'
+    -> cr' = Fr (Loc o' (pre' ++ [NT x]) suf') v''
+    -> stack_wf g (fr, cr :: frs)
+    -> unavailable_nts_are_open_calls g av (lstackOf (fr, cr :: frs))
+    -> unavailable_nts_are_open_calls g (NtSet.add x av) (lstackOf (cr', frs)).
+Proof.
+  intros g av fr cr cr' frs o o' pre pre' x suf' v v' v'' ? ? ? hw hu; subst; sis.
+  intros x' hi hn.
+  assert (hn' : ~ NtSet.In x' av) by ND.fsetdec.
+  apply hu in hn'; auto.
+  destruct hn' as [hng [frs_pre [cr [frs_suf [suf [heq [ha heq']]]]]]].
+  destruct frs_pre as [| fr_pre frs_pre]; inv heq; inv ha; sis.
+  - inv heq'; ND.fsetdec.
+  - split; eauto 8.
+    inv hw; rewrite app_nil_r in *.
+    apply nullable_app; eauto.
+Qed.
+
+Lemma push_preserves_unavailable_nts_invar :
+  forall g av fr ce o o' pre suf suf' x v v' frs,
+    fr    = Fr (Loc o pre (NT x :: suf)) v
+    -> ce = Fr (Loc o' [] suf') v'
+    -> unavailable_nts_are_open_calls g av (lstackOf (fr, frs))
+    -> unavailable_nts_are_open_calls g (NtSet.remove x av) (lstackOf (ce, fr :: frs)).
+Proof.
+  intros g av fr ce o o' pre suf suf' x v v' frs ? ? hu; subst; sis.
+  intros x' hi hn; split; auto.
+  destruct (NF.eq_dec x' x); subst.
+  - exists []; repeat eexists; eauto.
+  - assert (hn' : ~ NtSet.In x' av) by ND.fsetdec.
+    apply hu in hn'; auto.
+    destruct hn' as [? [frs_pre [? [? [? [heq [? ?]]]]]]]; subst; rewrite heq.
+    exists (Loc o pre (NT x :: suf) :: frs_pre); repeat eexists; eauto.
+Qed.
+    
+Lemma step_preserves_unavailable_nts_invar :
+  forall g st st',
+    step g st = StepK st'
+    -> stack_wf g st.(stack)
+    -> unavailable_nts_invar g st
+    -> unavailable_nts_invar g st'.
+Proof.
+  intros g [av stk ts] [av' stk' ts'] hs hw hu.
+  unfold unavailable_nts_invar in *.
+  unfold step in hs; dmeqs h; tc; inv hs.
+  - eapply return_preserves_unavailable_nts_invar; eauto. 
+  - intros x hi hn; ND.fsetdec.
+  - eapply push_preserves_unavailable_nts_invar; eauto.
+  - eapply push_preserves_unavailable_nts_invar; eauto.
+Qed.
+
+(* THE STACK SYMBOLS THAT HAVE ALREADY BEEN PROCESSED REPRESENT
+   A (PARTIAL) DERIVATION; THIS PREDICATE RELATES THOSE SYMBOLS
+   TO THE WORD (PREFIX) INVOLVED IN THE DERIVATION. *)
 Inductive stack_derivation (g : grammar) : parser_stack -> list token -> Prop :=
 | SD_nil :
     forall xo pre suf v w,
@@ -471,7 +542,7 @@ Inductive stack_derivation (g : grammar) : parser_stack -> list token -> Prop :=
 
 Hint Constructors stack_derivation.
 
-(* tactic for inverting a stack_derivation hypothesis *)
+(* Tactic for inverting a stack_derivation hypothesis *)
 Ltac inv_sd hsd wpre wsuf hgd hsd' := inversion hsd as [? ? ? ? wpre hgd | ? ? ? ? ? ? wpre wsuf hgd hsd']; subst; clear hsd.
 
 (* Parser invariant: the processed stack symbols represent a 
@@ -504,149 +575,4 @@ Lemma stack_derivation_cases :
 Proof.
   intros g fr frs w hsd.
   destruct frs as [| fr' frs]; inv hsd; eauto.
-Qed.
-
-(* another invariant *)
-
-Definition nt_unavailable (g : grammar) (x : nonterminal) (av : NtSet.t) : Prop :=
-  In x (lhss g) /\ ~ NtSet.In x av.
-
-Definition processed_symbols_all_nullable (g : grammar) (frs : list frame) : Prop :=
-  Forall (fun fr => nullable_gamma g fr.(loc).(rpre)) frs.
-
-Hint Constructors Forall.
-
-Definition unavailable_nts_are_open_calls_invar g st : Prop :=
-  match st with
-  | Pst av (fr, frs) _ =>
-    forall (x : nonterminal),
-      nt_unavailable g x av
-      -> nullable_gamma g fr.(loc).(rpre)
-         /\ (exists frs_pre fr_cr frs_suf suf,
-                frs = frs_pre ++ fr_cr :: frs_suf
-                /\ processed_symbols_all_nullable g frs_pre
-                /\ fr_cr.(loc).(rsuf) = NT x :: suf)
-  end.
-
-Lemma all_nts_available_no_nt_unavailable :
-  forall g x,
-    ~ nt_unavailable g x (allNts g).
-Proof.
-  unfold not; unfold nt_unavailable; intros g x [hi hn].
-  apply in_lhss_iff_in_allNts in hi; auto.
-Qed.
-
-Lemma unavailable_nts_invar_starts_true :
-  forall g ys ts,
-    unavailable_nts_are_open_calls_invar g (mkInitState g ys ts).
-Proof.
-  intros g ys ts; unfold mkInitState; unfold unavailable_nts_are_open_calls_invar.
-  intros x hn.
-  apply all_nts_available_no_nt_unavailable in hn; inv hn.
-Qed.
-
-Lemma nt_unavailable_add :
-  forall g x x' av,
-    nt_unavailable g x' (NtSet.add x av)
-    -> x' <> x /\ nt_unavailable g x' av.
-Proof.
-  intros g x x' av hn.
-  destruct (NF.eq_dec x' x); subst.
-  - unfold nt_unavailable in hn; ND.fsetdec.
-  - unfold nt_unavailable in *; destruct hn as [hi hn].
-    repeat split; auto.
-    ND.fsetdec.
-Qed.
-
-Lemma nt_unavailable_remove :
-  forall g x x' av,
-    nt_unavailable g x' (NtSet.remove x av)
-    -> x' <> x
-    -> nt_unavailable g x' av.
-Proof.
-  intros g x x' av hn hneq.
-  destruct hn as [hi hn].
-  split; auto.
-  ND.fsetdec.
-Qed.
-
-Lemma step_preserves_unavailable_nts_invar :
-  forall g st st',
-    step g st = StepK st'
-    -> stack_wf g st.(stack)
-    -> unavailable_nts_are_open_calls_invar g st
-    -> unavailable_nts_are_open_calls_invar g st'.
-Proof.
-  intros g st st' hs hw hu.
-  destruct st as [av (fr, frs) ts].
-  destruct fr as [[xo pre suf] v]; sis.
-  destruct suf as [| [a | x] suf].
-  - destruct frs as [| [[xo_prev pre_prev suf_prev] v_prev] frs].
-    + destruct ts; tc.
-    + destruct suf_prev as [| [a | x] suf_prev]; tc; inv hs.
-      unfold unavailable_nts_are_open_calls_invar; sis.
-      intros x' hn.
-      apply nt_unavailable_add in hn; destruct hn as [hneq hn].
-      apply hu in hn; clear hu.
-      destruct hn as [hng [frs_pre [fr_cr [frs_suf [suf [heq [hall heq']]]]]]].
-      destruct frs_pre as [| fr_pre frs_pre]; sis.
-      * inv heq; sis.
-        inv heq'; tc.
-      * inv heq. 
-        inv hall; sis.
-        split.
-        -- apply nullable_app; auto.
-           constructor; auto.
-           inv hw; rewrite app_nil_r in *.
-           econstructor; eauto.
-        -- repeat eexists; repeat split; eauto.
-  - destruct ts as [| (a', l) ts]; tc.
-    destruct (t_eq_dec a' a); tc; subst; inv hs.
-    (* lemma *)
-    unfold unavailable_nts_are_open_calls_invar; sis.
-    intros x hn.
-    apply all_nts_available_no_nt_unavailable in hn; inv hn.
-  - destruct (NtSet.mem x av) eqn:hm; tc.
-    destruct (llPredict g x _) as [rhs | rhs | | m] eqn:hl; inv hs.
-    + unfold unavailable_nts_are_open_calls_invar; sis.
-      intros x' hn.
-      split; auto.
-      destruct (NF.eq_dec x' x); subst.
-      * exists [].
-        exists (Fr (Loc xo pre (NT x :: suf)) v).
-        exists frs.
-        exists suf.
-        sis.
-        repeat split; auto.
-        constructor.
-      * apply nt_unavailable_remove in hn; auto. 
-        apply hu in hn.
-        destruct hn as [hng [frs_pre [fr_cr [frs_suf [suf' [heq [hall heq']]]]]]]; subst.
-        exists ((Fr (Loc xo pre (NT x :: suf)) v) :: frs_pre).
-        exists fr_cr.
-        exists frs_suf.
-        exists suf'.
-        repeat split; auto.
-        constructor; auto.
-    +  unfold unavailable_nts_are_open_calls_invar; sis.
-      intros x' hn.
-      split; auto.
-      destruct (NF.eq_dec x' x); subst.
-      * exists [].
-        exists (Fr (Loc xo pre (NT x :: suf)) v).
-        exists frs.
-        exists suf.
-        sis.
-        repeat split; auto.
-        constructor.
-      * apply nt_unavailable_remove in hn; auto. 
-        apply hu in hn.
-        destruct hn as [hng [frs_pre [fr_cr [frs_suf [suf' [heq [hall heq']]]]]]]; subst.
-        exists ((Fr (Loc xo pre (NT x :: suf)) v) :: frs_pre).
-        exists fr_cr.
-        exists frs_suf.
-        exists suf'.
-        repeat split; auto.
-        constructor; auto.
-    + destruct (NtSet.mem x (allNts g)); tc.
 Qed.
