coq/Parser_error_free_termination.v
@@ -1,9 +1,11 @@
 Require Import List.
 Require Import GallStar.Defs.
 Require Import GallStar.Lex.
+Require Import GallStar.Prediction.
 Require Import GallStar.Parser.
 Require Import GallStar.Tactics.
 Require Import GallStar.Utils.
+Require Import GallStar.Prediction_error_free_termination.
 Import ListNotations.
 
 (* The parser never reaches an invalid state;
@@ -60,123 +62,6 @@ Proof.
   - constructor.
 Qed.
 
-Inductive nullable_frames_path (g : grammar) : nonterminal -> nonterminal -> list frame -> Prop :=
-| NFP : 
-    forall top_fr mid_frs bot_fr x y suf suf',
-      bot_fr.(loc).(rsuf) = NT x :: suf
-      -> List.Forall (fun mf => nullable_gamma g mf.(loc).(rpre)) mid_frs
-      -> nullable_gamma g top_fr.(loc).(rpre)
-      -> top_fr.(loc).(rsuf) = NT y :: suf'
-      -> nullable_frames_path g x y (top_fr :: mid_frs ++ [bot_fr]).
-
-Lemma nullable_path_two_head_frames :
-  forall g l l' v v' frs y suf,
-    frames_wf g (Fr l v :: Fr l' v' :: frs)
-    -> nullable_gamma g l.(rpre)
-    -> l.(rsuf) = NT y :: suf
-    -> exists x suf',
-        l'.(rsuf) = NT x :: suf'
-        /\ nullable_path g (NT x) (NT y).
-Proof.
-  intros g l l' v v' frs y suf hw hn heq.
-  inv hw; sis; subst; eauto.
-Qed.
-(*
-Lemma nullable_path_two_head_frames :
-  forall g fr fr' frs y suf,
-    frames_wf g (fr :: fr' :: frs)
-    -> nullable_gamma g fr.(loc).(rpre)
-    -> fr.(loc).(rsuf) = NT y :: suf
-    -> exists x suf',
-        fr'.(loc).(rsuf) = NT x :: suf'
-        /\ nullable_path g (NT x) (NT y).
-Proof.
-  intros g fr fr' frs y suf hw hn heq.
-  unfold frames_wf in hw.
-  sis.
-  inv hw; sis; subst.
-  assert (suf' = NT y :: suf).
-  { rewrite <- H in heq; sis; auto. }
-  subst.
-  exists x; exists suf0; split; eauto.
-  eapply DirectPath; eauto.
-  rewrite <- H in heq.
-  simpl in heq; subst.
-  eauto.
-  destruct fr as rewrit
-  destruct fr.
-  exists x; exists suf0; split; auto.
-  econstructor; eauto.
-Qed.
-
-Lemma nullable_path_two_head_frames :
-  forall g fr fr' frs y suf,
-    frames_wf g (fr :: fr' :: frs)
-    -> nullable_gamma g fr.(loc).(rpre)
-    -> fr.(loc).(rsuf) = NT y :: suf
-    -> exists x suf',
-        fr'.(loc).(rsuf) = NT x :: suf'
-        /\ nullable_path g (NT x) (NT y).
-Proof.
-  intros g fr fr' frs y suf hw hn heq.
-  unfold frames_wf in *; sis.
-  inv hw; sis; subst; eauto 20.  
-Qed.
-
-*)
-
-(* CLEAN THIS UP *)
-Lemma stack_configuration_repr_nullable_path :
-  forall g frs l l_cr v v_cr x y suf suf',
-    frames_wf g (Fr l v :: frs ++ [Fr l_cr v_cr])
-    -> nullable_gamma g l.(rpre)
-    -> l.(rsuf) = NT y :: suf
-    -> processed_symbols_all_nullable g frs
-    -> l_cr.(rsuf) = NT x :: suf'
-    -> nullable_path g (NT x) (NT y).
-Proof.
-  intros g frs.
-  induction frs as [| (l', v') frs IH]; intros l l_cr v v_cr x y suf suf' hw hn heq hp heq'; sis. 
-  - inv hw; sis.
-    inv heq'.
-    eapply DirectPath; eauto.
-  - rename y into z.
-    pose proof hw as hw'.
-    eapply nullable_path_two_head_frames in hw'; eauto.
-    destruct hw' as [y [suf'' [heq'' hnp]]].
-    apply nullable_path_trans with (y := (NT y)); auto.
-    apply frames_wf_tl in hw.
-    inv hp; sis.
-    eapply IH in hw; eauto.
-Qed.
-
-(*
-Lemma stack_configuration_repr_nullable_path :
-  forall g frs fr fr_cr x y suf suf',
-    frames_wf g (fr :: frs ++ [fr_cr])
-    -> nullable_gamma g fr.(loc).(rpre)
-    -> fr.(loc).(rsuf) = NT y :: suf
-    -> processed_symbols_all_nullable g frs
-    -> fr_cr.(loc).(rsuf) = NT x :: suf'
-    -> nullable_path g (NT x) (NT y).
-Proof.
-  intros g frs.
-  induction frs as [| fr' frs IH]; intros fr fr_cr x y suf suf' hw hn heq hp heq'; sis.
-  - inv hw; sis.
-    inv heq'.
-    eapply DirectPath; eauto.
-  - rename y into z.
-    pose proof hw as hw'.
-    eapply nullable_path_two_head_frames in hw'; eauto.
-    destruct hw' as [y [suf'' [heq'' hnp]]].
-    apply nullable_path_trans with (y := (NT y)); auto.
-    assert (hw' : frames_wf g (fr' :: frs ++ [fr_cr])).
-    { inv hw; auto. }
-    inv hp.
-    eapply IH in hw'; eauto.
-Qed.
- *)
-
 (* CLEAN UP *)
 Lemma multistep_left_recursion_detection_sound :
   forall (g      : grammar)
@@ -187,7 +72,7 @@ Lemma multistep_left_recursion_detection_sound :
          (x      : nonterminal),
     tri = meas g st
     -> stack_wf g st.(stack)
-    -> unavailable_nts_are_open_calls_invar g st
+    -> unavailable_nts_invar g st
     -> multistep g st a' = Error (LeftRecursion x)
     -> left_recursive g (NT x).
 Proof.
@@ -200,22 +85,18 @@ Proof.
     destruct st as [av (fr, frs) ts].
     apply step_LeftRecursion_facts in hs.
     destruct hs as [hnin [hin [suf heq]]]; subst.
-    unfold unavailable_nts_are_open_calls_invar in hu.
-    unfold nt_unavailable in hu.
-    assert (hand : In x (lhss g) /\ ~ NtSet.In x av).
-    { split; auto.
-      apply in_lhss_iff_in_allNts; auto. }
-    apply hu in hand; clear hu.
-    destruct hand as [hng [frs_pre [fr_cr [frs_suf [suf_cr [heq' [hp heq'']]]]]]]; subst.
-    simpl in hw.
-    assert (happ : fr :: frs_pre ++ fr_cr :: frs_suf =
-                   (fr :: frs_pre ++ [fr_cr]) ++ frs_suf).
+    unfold unavailable_nts_invar in hu.
+    apply hu in hnin; auto.
+    destruct hnin as [hng [frs_pre [fr_cr [frs_suf [suf_cr [heq' [hp heq'']]]]]]]; subst.
+    simpl in hw. unfold frames_wf in hw; simpl in hw.
+    rewrite heq' in hw.
+    assert (happ : loc fr :: frs_pre ++ fr_cr :: frs_suf =
+                   (loc fr :: frs_pre ++ [fr_cr]) ++ frs_suf).
     (* lemma *)
     { simpl. rewrite <- app_assoc. simpl. auto. }
     rewrite happ in hw; clear happ.
-    apply frames_wf_app_l in hw.
-    destruct fr as (l, v); destruct fr_cr as (l', v').
-    eapply stack_configuration_repr_nullable_path in hw; eauto.
+    apply Prediction.locations_wf_app_l in hw.
+    eapply Prediction_error_free_termination.stack_configuration_repr_nullable_path in hw; eauto.
   - eapply IH with (y := meas g st'); eauto.
     + eapply step_meas_lt; eauto.
     + (* redefine invariants to get rid of these destructs *)
@@ -236,10 +117,8 @@ Proof.
     constructor.
   - (* lemma *)
     unfold mkInitState.
-    unfold unavailable_nts_are_open_calls_invar; simpl.
-    intros x' hu.
-    exfalso.
-    eapply all_nts_available_no_nt_unavailable; eauto.
+    unfold unavailable_nts_invar; simpl.
+    intros; ND.fsetdec.
 Qed.
   
 Lemma parser_doesn't_find_left_recursion_in_non_left_recursive_grammar :
@@ -253,9 +132,6 @@ Proof.
   intros g ss ts x hn; unfold not; intros hp.
   apply parse_left_recursion_detection_sound in hp; firstorder.
 Qed.
-
-Require Import GallStar.Prediction.
-Require Import GallStar.Prediction_error_free_termination.
 
 Lemma parse_never_returns_prediction_error :
   forall (g : grammar)
